Several Things & Machine Integer WIP

Phi_Semantics/PhiSem_Machine_Integer.thy
@@ -1,5 +1,5 @@
 theory PhiSem_Machine_Integer
-  imports PhiSem_Common_Int PhiSem_Generic_Boolean
+  imports PhiSem_Common_Int PhiSem_Generic_Boolean "HOL-Library.Word"
 begin
 
 chapter \<open>Semantics for Machine Integers\<close>
@@ -11,10 +11,6 @@ subsubsection \<open>Type\<close>
 virtual_datatype \<phi>machine_int_ty = \<phi>empty_ty +
   T_int     :: nat \<comment> \<open>in unit of bits\<close>
 
-context \<phi>machine_int_ty begin
-abbreviation int where \<open>int \<equiv> T_int.mk\<close>
-end
-
 debt_axiomatization T_int :: \<open>nat type_entry\<close>
   where \<phi>machine_int_ty_ax: \<open>\<phi>machine_int_ty TY_CONS_OF T_int\<close>
 
@@ -23,6 +19,26 @@ interpretation \<phi>machine_int_ty TY_CONS_OF _ _ T_int using \<phi>machine_int
 hide_fact \<phi>machine_int_ty_ax \<phi>machine_int_ty_axioms \<phi>machine_int_ty_names_def \<phi>machine_int_ty_def
   \<phi>machine_int_ty_prjs_axioms \<phi>machine_int_ty_prjs_def \<phi>machine_int_ty.axioms \<phi>machine_int_ty.intro
   \<phi>machine_int_ty__names.\<phi>machine_int_ty_names_axioms \<phi>machine_int_ty_prjs.axioms
+
+syntax "_int_semty_" :: \<open>type \<Rightarrow> TY\<close> ("int'(_')")
+
+translations "int('b)" <= "CONST T_int.mk LENGTH('b)"
+
+ML \<open>local open Ast in
+  fun need_add_sort (Appl [Constant \<^syntax_const>\<open>_ofsort\<close>, Variable _, _]) = true
+    | need_add_sort (Variable _) = true
+    | need_add_sort _ = false
+  fun add_sort X =
+    if need_add_sort X
+    then Appl [Constant \<^syntax_const>\<open>_ofsort\<close>, X, Constant \<^class_syntax>\<open>len\<close>]
+    else X
+end\<close>
+
+parse_ast_translation \<open>
+  let open Ast
+   in [(\<^syntax_const>\<open>_int_semty_\<close>, (fn _ => fn [V] =>
+          Appl [Constant \<^const_syntax>\<open>T_int.mk\<close>, Appl [Constant \<^syntax_const>\<open>_type_length\<close>, add_sort V]]))] end\<close>
+
 
 subsubsection \<open>Value\<close>
 
@@ -39,13 +55,13 @@ hide_fact \<phi>machine_int_val_ax \<phi>machine_int_val_axioms
 subsubsection \<open>Semantics\<close>
 
 debt_axiomatization
-    WT_int[simp]: \<open>Well_Type (int b)     = { V_int.mk (b,x)    |x. x < 2 ^ Big b } \<close>
+    WT_int[simp]: \<open>Well_Type (T_int.mk b)     = { V_int.mk (b,x)    |x. x < 2 ^ b } \<close>
 and can_eqcmp_int[simp]: "Can_EqCompare res (V_int.mk (b1,x1)) (V_int.mk (b2,x2)) \<longleftrightarrow> b1 = b2"
 and eqcmp_int[simp]: "EqCompare (V_int.mk i1) (V_int.mk i2) \<longleftrightarrow> i1 = i2"
-and  zero_int[simp]: \<open>Zero (int b)    = Some (V_int.mk (b,0))\<close>
+and  zero_int[simp]: \<open>Zero (T_int.mk b)    = Some (V_int.mk (b,0))\<close>
 
 lemma Valid_Types[simp]:
-  \<open>Valid_Type (int n)\<close>
+  \<open>Valid_Type (T_int.mk n)\<close>
   unfolding Inhabited_def
   apply simp
   using less_exp by blast
@@ -55,106 +71,151 @@ section \<open>\<phi>-Types\<close>
 
 subsection \<open>Integer\<close>
 
-subsubsection \<open>Natural Nmbers\<close>
+subsubsection \<open>Words\<close>
+
+definition Word :: \<open>'b itself \<Rightarrow> (VAL, 'b::len word) \<phi>\<close>
+  where \<open>Word _ x = { V_int.mk (LENGTH('b), unat x) }\<close>
+
+syntax Word_syntax :: "type \<Rightarrow> (VAL, 'b::len word) \<phi>" ("Word'(_')")
+
+translations "Word('x)" <= "CONST Word TYPE('x)"
+
+parse_ast_translation \<open>
+  let open Ast
+   in [(\<^syntax_const>\<open>Word_syntax\<close>, (fn _ => fn [V] =>
+          Appl [Constant \<^const_syntax>\<open>Word\<close>, Appl [Constant \<^syntax_const>\<open>_TYPE\<close>, add_sort V]]))] end\<close>
+
+
+
+lemma Word_expn[\<phi>expns]:
+  \<open>p \<in> (x \<Ztypecolon> Word('b)) \<longleftrightarrow> p = V_int.mk (LENGTH('b), unat x)\<close>
+  unfolding \<phi>Type_def Word_def by simp
+
+lemma [elim!,\<phi>inhabitance_rule]:
+  \<open>Inhabited (x \<Ztypecolon> Word('b)) \<Longrightarrow> C \<Longrightarrow> C\<close> .
+
+lemma [\<phi>reason 1000]:
+  \<open>\<phi>SemType (x \<Ztypecolon> Word('b)) int('b)\<close>
+  unfolding \<phi>SemType_def subset_iff by (simp add: Word_expn)
+
+lemma [\<phi>reason 1000]:
+  "\<phi>Equal Word('b) (\<lambda>x y. True) (=)"
+  unfolding \<phi>Equal_def by (simp add: word_unat_eq_iff Word_expn)
+
+lemma [\<phi>reason 1000]:
+  "\<phi>Zero int('b) Word('b) (0::'b::len word)"
+  unfolding \<phi>Zero_def by (simp add: Word_expn image_iff)
+
+
+
+subsubsection \<open>Natural Numbers\<close>
 
 paragraph \<open>Natural Number\<close>
 
-definition \<phi>Nat :: "nat \<Rightarrow> (VAL, nat) \<phi>" ("\<nat>[_]")
-  where "\<nat>[b] x = (if x < 2^b then { V_int.mk (b,x) } else {})"
+definition \<phi>Nat :: "'b::len itself \<Rightarrow> (VAL, nat) \<phi>"
+  where [\<phi>defs]: "\<phi>Nat _ x = ((of_nat x :: 'b word) \<Ztypecolon> Word('b) \<^bold>s\<^bold>u\<^bold>b\<^bold>j x \<in> {0..< 2 ^ LENGTH('b)})"
 
-lemma \<phi>Nat_expn[\<phi>expns]:
-  "p \<in> (x \<Ztypecolon> \<nat>[b]) \<longleftrightarrow> (p = V_int.mk (b,x)) \<and> x < 2 ^ Big b"
-  unfolding \<phi>Type_def Big_def by (simp add: \<phi>Nat_def)
+syntax \<phi>Nat_syntax :: "type \<Rightarrow> (VAL, nat) \<phi>" ("\<nat>'(_')")
 
-lemma \<phi>Nat_elim[elim!,\<phi>inhabitance_rule]:
-  "Inhabited (x \<Ztypecolon> \<nat>[b]) \<Longrightarrow> (x < 2 ^ Big b \<Longrightarrow> C) \<Longrightarrow> C"
-  unfolding Inhabited_def by (simp add: \<phi>expns)
+translations "\<nat>('x)" <= "CONST \<phi>Nat TYPE('x)"
 
-lemma \<open>Inhabited (x \<Ztypecolon> \<nat>[b]) \<longleftrightarrow> x < 2^Big b\<close>
-  unfolding Inhabited_def by (simp add: \<phi>expns)
+parse_ast_translation \<open>
+  let open Ast
+   in [(\<^syntax_const>\<open>\<phi>Nat_syntax\<close>, (fn _ => fn [V] =>
+          Appl [Constant \<^const_syntax>\<open>\<phi>Nat\<close>, Appl [Constant \<^syntax_const>\<open>_TYPE\<close>, add_sort V]]))] end\<close>
 
-lemma \<phi>Nat_semty[\<phi>reason 1000]:
-  \<open>\<phi>SemType (x \<Ztypecolon> \<nat>[b]) (int b)\<close>
-  unfolding \<phi>SemType_def subset_iff by (simp add: \<phi>expns Big_def)
 
-lemma [\<phi>reason 1000]:
-  "\<phi>Equal (\<nat>[b]) (\<lambda>x y. True) (=)"
-  unfolding \<phi>Equal_def by (auto simp add: \<phi>expns)
+lemma [\<phi>reason 800]:
+  \<open> \<^bold>p\<^bold>r\<^bold>e\<^bold>m\<^bold>i\<^bold>s\<^bold>e y = of_nat x \<Longrightarrow> x \<Ztypecolon> \<nat>('b) \<^bold>i\<^bold>m\<^bold>p\<^bold>l\<^bold>i\<^bold>e\<^bold>s y \<Ztypecolon> Word('b) \<^bold>a\<^bold>n\<^bold>d x < 2 ^ LENGTH('b)\<close>
+  for y :: \<open>'b::len word\<close>
+  \<medium_left_bracket> destruct\<phi> _ \<medium_right_bracket>. .
 
-lemma [\<phi>reason 1000]:
-  "\<phi>Zero (int b) (\<nat>[b]) 0" unfolding \<phi>Zero_def by (simp add: \<phi>expns)
+lemma [
+  \<phi>reason 800 for \<open>_ \<Ztypecolon> \<phi>Nat _ \<^bold>i\<^bold>m\<^bold>p\<^bold>l\<^bold>i\<^bold>e\<^bold>s _ \<^bold>a\<^bold>n\<^bold>d _ @action to (Word _)\<close>,
+  \<phi>inhabitance_rule
+]:
+  \<open>x \<Ztypecolon> \<nat>('b) \<^bold>i\<^bold>m\<^bold>p\<^bold>l\<^bold>i\<^bold>e\<^bold>s (of_nat x :: 'b::len word) \<Ztypecolon> Word('b) \<^bold>a\<^bold>n\<^bold>d x < 2 ^ LENGTH('b)
+   @action to Word('b)\<close>
+  \<medium_left_bracket> \<medium_right_bracket>. .
 
-lemma [\<phi>reason]:
-  \<open> \<^bold>p\<^bold>r\<^bold>e\<^bold>m\<^bold>i\<^bold>s\<^bold>e x < 2^Big b
-\<Longrightarrow> is_singleton (x \<Ztypecolon> \<nat>[b])\<close>
-  by (rule is_singletonI''; simp add: \<phi>expns)
 
-paragraph \<open>Rounded Natural Number\<close>
+lemma [\<phi>reason 1200]:
+  \<open> \<^bold>p\<^bold>r\<^bold>e\<^bold>m\<^bold>i\<^bold>s\<^bold>e y = unat x \<Longrightarrow> x \<Ztypecolon> Word('b) \<^bold>i\<^bold>m\<^bold>p\<^bold>l\<^bold>i\<^bold>e\<^bold>s y \<Ztypecolon> \<nat>('b)\<close>
+  for x :: \<open>'b::len word\<close>
+  \<medium_left_bracket> construct\<phi> \<open>unat x \<Ztypecolon> \<nat>('b)\<close> \<medium_right_bracket>. .
 
-definition \<phi>NatRound :: "nat \<Rightarrow> (VAL, nat) \<phi>" ("\<nat>\<^sup>r[_]")
-  where "\<nat>\<^sup>r[b] x = { V_int.mk (b, (x mod 2 ^ Big b)) }"
-
-lemma \<phi>NatRound_expn[\<phi>expns]:
-  "p \<in> (x \<Ztypecolon> \<nat>\<^sup>r[b]) \<longleftrightarrow> p = V_int.mk (b, (x mod 2 ^ Big b))"
-  unfolding \<phi>Type_def \<phi>NatRound_def by simp
-
-lemma \<open>Inhabited (x \<Ztypecolon> \<nat>\<^sup>r[b]) \<longleftrightarrow> True\<close>
-  unfolding Inhabited_def by (auto simp add: \<phi>expns)
+lemma [\<phi>reason 1200 for \<open>_ \<Ztypecolon> Word _ \<^bold>i\<^bold>m\<^bold>p\<^bold>l\<^bold>i\<^bold>e\<^bold>s _ \<^bold>a\<^bold>n\<^bold>d _ @action to (\<phi>Nat _)\<close>]:
+  \<open> x \<Ztypecolon> Word('b) \<^bold>i\<^bold>m\<^bold>p\<^bold>l\<^bold>i\<^bold>e\<^bold>s unat x \<Ztypecolon> \<nat>('b) @action to \<nat>('b)\<close>
+  for x :: \<open>'b::len word\<close> \<medium_left_bracket> \<medium_right_bracket>. .
 
 lemma [\<phi>reason 1000]:
-  "\<phi>Zero (int b) (\<nat>\<^sup>r[b]) 0"
-  unfolding \<phi>Zero_def by (simp add: \<phi>expns)
-
-lemma \<phi>NatRound_semty[\<phi>reason 1000]:
-  \<open>\<phi>SemType (x \<Ztypecolon> \<nat>\<^sup>r[b]) (int b)\<close>
-  unfolding \<phi>SemType_def subset_iff by (simp add: \<phi>expns)
+  "\<phi>Equal (\<nat>('b::len)) (\<lambda>x y. True) (=)"
+  \<medium_left_bracket> to \<open>Word('b)\<close> \<medium_right_bracket> using \<phi>lemmata of_nat_inverse by blast .
 
 
 subsection \<open>Integer\<close>
 
-definition \<phi>Int :: "nat \<Rightarrow> (VAL, int) \<phi>" ("\<int>[_]")
-  where "\<phi>Int b x =(if x < 2^(b - 1) \<and> -(2^(b-1)) \<le> x \<and> (b = 0 \<longrightarrow> x = 0)
-                    then { V_int.mk (b, (if x \<ge> 0 then nat x else nat (2^b + x))) }
-                    else {})"
+definition \<phi>Int :: "'b::len itself \<Rightarrow> (VAL, int) \<phi>"
+  where [\<phi>defs]: "\<phi>Int _ x = ((of_int x :: 'b word) \<Ztypecolon> Word('b)
+                              \<^bold>s\<^bold>u\<^bold>b\<^bold>j x \<in> { -(2^(LENGTH('b)-1)) ..< 2^(LENGTH('b)-1)})"
 
-lemma \<phi>Int_expn[\<phi>expns]:
-  "p \<in> (x \<Ztypecolon> \<int>[b]) \<longleftrightarrow> p = V_int.mk (b, (if x \<ge> 0 then nat x else nat (2^b + x)))
-                      \<and> x < 2^(b - 1) \<and> -(2^(b-1)) \<le> x \<and> (b = 0 \<longrightarrow> x = 0)"
-  unfolding \<phi>Type_def by (simp add: \<phi>Int_def)
+syntax \<phi>Int_syntax :: "type \<Rightarrow> (VAL, nat) \<phi>" ("\<int>'(_')")
 
-lemma \<phi>Int_inhabited[elim!,\<phi>inhabitance_rule]:
-  "Inhabited (x \<Ztypecolon> \<int>[b]) \<Longrightarrow> (x < 2^(b - 1) \<and> -(2^(b-1)) \<le> x \<and> (b = 0 \<longrightarrow> x = 0) \<Longrightarrow> C) \<Longrightarrow> C"
-  unfolding Inhabited_def by (simp add: \<phi>expns) 
+translations "\<int>('x)" == "CONST \<phi>Int TYPE('x)"
 
-lemma [simp]: \<open>- (2^(b - 1)) \<le> x \<Longrightarrow> 0 \<le> 2 ^ b + x\<close> for x :: int
-  by (smt (verit, best) diff_le_self power_increasing_iff)
+parse_ast_translation \<open>
+  let open Ast
+   in [(\<^syntax_const>\<open>\<phi>Int_syntax\<close>, (fn _ => fn [V] =>
+          Appl [Constant \<^const_syntax>\<open>\<phi>Int\<close>, Appl [Constant \<^syntax_const>\<open>_TYPE\<close>, add_sort V]]))] end\<close>
+
+lemma [\<phi>reason 800]:
+  " \<^bold>p\<^bold>r\<^bold>e\<^bold>m\<^bold>i\<^bold>s\<^bold>e y = of_int x
+\<Longrightarrow> x \<Ztypecolon> \<int>('b) \<^bold>i\<^bold>m\<^bold>p\<^bold>l\<^bold>i\<^bold>e\<^bold>s y \<Ztypecolon> Word('b) \<^bold>a\<^bold>n\<^bold>d x \<in> { -(2^(LENGTH('b)-1)) ..< 2^(LENGTH('b)-1)}"
+  \<medium_left_bracket> destruct\<phi> _ \<medium_right_bracket>. .
+
+lemma [
+  \<phi>reason 800 for \<open>_ \<Ztypecolon> \<int>(_) \<^bold>i\<^bold>m\<^bold>p\<^bold>l\<^bold>i\<^bold>e\<^bold>s _ \<^bold>a\<^bold>n\<^bold>d _ @action to Word(_)\<close>,
+  \<phi>inhabitance_rule
+]:
+  \<open>x \<Ztypecolon> \<int>('b) \<^bold>i\<^bold>m\<^bold>p\<^bold>l\<^bold>i\<^bold>e\<^bold>s (of_int x :: 'b::len word) \<Ztypecolon> Word('b) \<^bold>a\<^bold>n\<^bold>d x \<in> { -(2^(LENGTH('b)-1)) ..< 2^(LENGTH('b)-1)}
+   @action to Word('b)\<close>
+  \<medium_left_bracket> \<medium_right_bracket>. .
+
+lemma [\<phi>reason 800 for \<open>?x \<Ztypecolon> Word(_) \<^bold>i\<^bold>m\<^bold>p\<^bold>l\<^bold>i\<^bold>e\<^bold>s _ \<Ztypecolon> \<int>(_) \<^bold>a\<^bold>n\<^bold>d _\<close>]:
+  " \<^bold>p\<^bold>r\<^bold>e\<^bold>m\<^bold>i\<^bold>s\<^bold>e y = sint x
+\<Longrightarrow> x \<Ztypecolon> Word('b) \<^bold>i\<^bold>m\<^bold>p\<^bold>l\<^bold>i\<^bold>e\<^bold>s y \<Ztypecolon> \<int>('b)"
+  for x :: \<open>'b::len word\<close>
+  \<medium_left_bracket> construct\<phi> \<open>y \<Ztypecolon> \<int>('b)\<close>
+    affirm apply (simp add: \<open>y = sint x\<close>) using sint_greater_eq sint_less by blast
+  \<medium_right_bracket>. .
+
+lemma [\<phi>reason 800 for \<open>_ \<Ztypecolon> Word(_) \<^bold>i\<^bold>m\<^bold>p\<^bold>l\<^bold>i\<^bold>e\<^bold>s _ @action to Word(_)\<close>]:
+  \<open> x \<Ztypecolon> Word('b) \<^bold>i\<^bold>m\<^bold>p\<^bold>l\<^bold>i\<^bold>e\<^bold>s sint x \<Ztypecolon> \<int>('b) @action to Word('b) \<close>
+  \<medium_left_bracket> \<medium_right_bracket>. .
+
+lemma [\<phi>reason 800 for \<open>_ \<Ztypecolon> \<int>(_) \<^bold>i\<^bold>m\<^bold>p\<^bold>l\<^bold>i\<^bold>e\<^bold>s _ @action to \<nat>(_)\<close>]:
+  \<open> \<^bold>p\<^bold>r\<^bold>e\<^bold>m\<^bold>i\<^bold>s\<^bold>e 0 \<le> x \<and> x < 2 ^ (LENGTH('b)-1)
+\<Longrightarrow> x \<Ztypecolon> \<int>('b) \<^bold>i\<^bold>m\<^bold>p\<^bold>l\<^bold>i\<^bold>e\<^bold>s nat x \<Ztypecolon> \<nat>('b) @action to \<nat>('b)\<close>
+  \<medium_left_bracket> to \<open>Word('b)\<close> \<medium_right_bracket>
+  by (smt (verit, ccfv_SIG) diff_le_self local.\<phi>(2) power_increasing_iff unat_eq_nat_uint word_of_int_inverse) .
+
+lemma [\<phi>reason 800 for \<open>_ \<Ztypecolon> \<nat>(_) \<^bold>i\<^bold>m\<^bold>p\<^bold>l\<^bold>i\<^bold>e\<^bold>s _ @action to \<int>(_)\<close>]:
+  \<open> \<^bold>p\<^bold>r\<^bold>e\<^bold>m\<^bold>i\<^bold>s\<^bold>e x < 2 ^ (LENGTH('b)-1)
+\<Longrightarrow> x \<Ztypecolon> \<nat>('b) \<^bold>i\<^bold>m\<^bold>p\<^bold>l\<^bold>i\<^bold>e\<^bold>s of_nat x \<Ztypecolon> \<int>('b) \<close>
+  \<medium_left_bracket> to \<open>Word('b)\<close> \<medium_right_bracket>
+  by (metis One_nat_def id_apply local.\<phi>(2) negative_zle of_int_eq_id of_nat_less_numeral_power_cancel_iff real_of_nat_eq_numeral_power_cancel_iff signed_of_nat signed_take_bit_int_eq_self_iff) .
 
 lemma [\<phi>reason 1000]:
-    "\<phi>Equal \<int>[b] (\<lambda>x y. True) (=)"
-  unfolding \<phi>Equal_def by (cases b) (auto simp add: \<phi>expns eq_nat_nat_iff)
+  \<open>\<phi>SemType (x \<Ztypecolon> \<int>('b)) int('b)\<close> \<medium_left_bracket> to \<open>Word(_)\<close> \<medium_right_bracket>. .
 
 lemma [\<phi>reason 1000]:
-    "\<phi>Zero (int b) \<int>[b] 0"
-  unfolding \<phi>Zero_def by (simp add: \<phi>expns)
+  "\<phi>Zero int('b) \<int>('b) 0" \<medium_left_bracket> \<open>0 \<Ztypecolon> Word('b)\<close> \<medium_right_bracket>. .
 
+lemma [\<phi>reason 1000]:
+  "\<phi>Equal \<int>('b) (\<lambda>x y. True) (=)"
+  \<medium_left_bracket> to \<open>Word(_)\<close> \<medium_right_bracket>
+  by (metis One_nat_def atLeastLessThan_iff local.\<phi>lemmata signed_take_bit_int_eq_self_iff sint_sbintrunc') .
 
-lemma \<phi>Int_semty[\<phi>reason 1000]:
-  \<open>\<phi>SemType (x \<Ztypecolon> \<int>[b]) (int b)\<close>
-  unfolding \<phi>SemType_def subset_iff
-  by (simp add: \<phi>expns Big_def) (smt (verit, ccfv_SIG) diff_le_self power_increasing_iff)
-
-
-subsubsection \<open>Subtyping\<close>
-
-lemma subty_Z_N[\<phi>overload nat]: 
-  "\<^bold>p\<^bold>r\<^bold>e\<^bold>m\<^bold>i\<^bold>s\<^bold>e 0 < x \<Longrightarrow> x \<Ztypecolon> \<int>[b] \<^bold>i\<^bold>m\<^bold>p\<^bold>l\<^bold>i\<^bold>e\<^bold>s nat x \<Ztypecolon> \<nat>[b]"
-  unfolding Imply_def Premise_def apply (simp add: \<phi>expns Big_def del: One_nat_def)
-  by (smt (verit, del_insts) diff_less less_numeral_extra(1) power_strict_increasing_iff)
-
-lemma subty_N_Z[\<phi>overload int]:
-  "\<^bold>p\<^bold>r\<^bold>e\<^bold>m\<^bold>i\<^bold>s\<^bold>e x < 2^(b - 1) \<Longrightarrow> x \<Ztypecolon> \<nat>[b] \<^bold>i\<^bold>m\<^bold>p\<^bold>l\<^bold>i\<^bold>e\<^bold>s Int.int x \<Ztypecolon> \<int>[b]"
-  unfolding Imply_def Premise_def apply (simp add: \<phi>expns Big_def del: One_nat_def)
-  by (metis less_one linorder_le_cases neg_0_le_iff_le not_exp_less_eq_0_int of_nat_0_le_iff order_trans power_0)
 
 
 section \<open>Instructions\<close>
@@ -175,64 +236,64 @@ definition op_const_int :: "nat \<Rightarrow> nat \<Rightarrow> VAL proc"
 definition op_add :: "nat \<Rightarrow> (VAL \<times> VAL, VAL) proc'"
   where "op_add bits =
       \<phi>M_caseV (\<lambda>vb va.
-      \<phi>M_getV (int bits) (snd o V_int.dest) vb (\<lambda>val_b.
-      \<phi>M_getV (int bits) (snd o V_int.dest) va (\<lambda>val_a.
+      \<phi>M_getV (T_int.mk bits) (snd o V_int.dest) vb (\<lambda>val_b.
+      \<phi>M_getV (T_int.mk bits) (snd o V_int.dest) va (\<lambda>val_a.
       Return (\<phi>arg (V_int.mk (bits, ((val_a + val_b) mod 2^bits))))
   )))"
 
 definition op_sub :: "nat \<Rightarrow> (VAL \<times> VAL, VAL) proc'"
   where "op_sub bits =
       \<phi>M_caseV (\<lambda>va vb.
-      \<phi>M_getV (int bits) (snd o V_int.dest) va (\<lambda>val_a.
-      \<phi>M_getV (int bits) (snd o V_int.dest) vb (\<lambda>val_b.
+      \<phi>M_getV (T_int.mk bits) (snd o V_int.dest) va (\<lambda>val_a.
+      \<phi>M_getV (T_int.mk bits) (snd o V_int.dest) vb (\<lambda>val_b.
       Return (\<phi>arg (V_int.mk (bits, ((2^bits + val_b - val_a) mod 2^bits))))
   )))"
 
 definition op_umul :: "nat \<Rightarrow> (VAL \<times> VAL, VAL) proc'"
   where "op_umul bits =
       \<phi>M_caseV (\<lambda>va vb.
-      \<phi>M_getV (int bits) (snd o V_int.dest) va (\<lambda>val_a.
-      \<phi>M_getV (int bits) (snd o V_int.dest) vb (\<lambda>val_b.
+      \<phi>M_getV (T_int.mk bits) (snd o V_int.dest) va (\<lambda>val_a.
+      \<phi>M_getV (T_int.mk bits) (snd o V_int.dest) vb (\<lambda>val_b.
       Return (\<phi>arg (V_int.mk (bits, ((val_b * val_a) mod 2^bits))))
   )))"
 
 definition op_udiv :: "nat \<Rightarrow> (VAL \<times> VAL, VAL) proc'"
   where "op_udiv bits =
       \<phi>M_caseV (\<lambda>va vb.
-      \<phi>M_getV (int bits) (snd o V_int.dest) va (\<lambda>val_a.
-      \<phi>M_getV (int bits) (snd o V_int.dest) vb (\<lambda>val_b.
+      \<phi>M_getV (T_int.mk bits) (snd o V_int.dest) va (\<lambda>val_a.
+      \<phi>M_getV (T_int.mk bits) (snd o V_int.dest) vb (\<lambda>val_b.
       Return (\<phi>arg (V_int.mk (bits, (val_b div val_a))))
   )))"
 
 definition op_lshr :: "nat \<Rightarrow> nat \<Rightarrow> (VAL \<times> VAL, VAL) proc'"
   where "op_lshr b_b b_a =
       \<phi>M_caseV (\<lambda>va vb.
-      \<phi>M_getV (int b_a) (snd o V_int.dest) va (\<lambda>val_a.
-      \<phi>M_getV (int b_b) (snd o V_int.dest) vb (\<lambda>val_b.
+      \<phi>M_getV (T_int.mk b_a) (snd o V_int.dest) va (\<lambda>val_a.
+      \<phi>M_getV (T_int.mk b_b) (snd o V_int.dest) vb (\<lambda>val_b.
       Return (\<phi>arg (V_int.mk (b_b, (val_b div 2 ^ val_a))))
   )))"
 
 definition op_lshl :: "nat \<Rightarrow> nat \<Rightarrow> (VAL \<times> VAL, VAL) proc'"
   where "op_lshl b_b b_a =
       \<phi>M_caseV (\<lambda>va vb.
-      \<phi>M_getV (int b_a) (snd o V_int.dest) va (\<lambda>val_a.
-      \<phi>M_getV (int b_b) (snd o V_int.dest) vb (\<lambda>val_b.
+      \<phi>M_getV (T_int.mk b_a) (snd o V_int.dest) va (\<lambda>val_a.
+      \<phi>M_getV (T_int.mk b_b) (snd o V_int.dest) vb (\<lambda>val_b.
       Return (\<phi>arg (V_int.mk (b_b, (val_b * 2 ^ val_a))))
   )))"
 
 definition op_lt :: "nat \<Rightarrow> (VAL \<times> VAL, VAL) proc'"
   where "op_lt bits =
       \<phi>M_caseV (\<lambda>va vb.
-      \<phi>M_getV (int bits) (snd o V_int.dest) va (\<lambda>val_a.
-      \<phi>M_getV (int bits) (snd o V_int.dest) vb (\<lambda>val_b.
+      \<phi>M_getV (T_int.mk bits) (snd o V_int.dest) va (\<lambda>val_a.
+      \<phi>M_getV (T_int.mk bits) (snd o V_int.dest) vb (\<lambda>val_b.
       Return (\<phi>arg (V_bool.mk (val_b < val_a)))
   )))"
 
 definition op_le :: "nat \<Rightarrow> (VAL \<times> VAL, VAL) proc'"
   where "op_le bits =
       \<phi>M_caseV (\<lambda>va vb.
-      \<phi>M_getV (int bits) (snd o V_int.dest) va (\<lambda>val_a.
-      \<phi>M_getV (int bits) (snd o V_int.dest) vb (\<lambda>val_b.
+      \<phi>M_getV (T_int.mk bits) (snd o V_int.dest) va (\<lambda>val_a.
+      \<phi>M_getV (T_int.mk bits) (snd o V_int.dest) vb (\<lambda>val_b.
       Return (\<phi>arg (V_bool.mk (val_b \<le> val_a)))
   )))"
 
@@ -248,10 +309,17 @@ bundle unfold_Big = Big_def[iff]
 
 subsubsection \<open>Constant Integer\<close>
 
-lemma op_const_int_\<phi>app:
-  \<open>\<^bold>p\<^bold>r\<^bold>e\<^bold>m\<^bold>i\<^bold>s\<^bold>e n < 2 ^ Big b \<Longrightarrow> \<^bold>p\<^bold>r\<^bold>o\<^bold>c op_const_int b n \<lbrace> Void \<longmapsto> \<^bold>v\<^bold>a\<^bold>l n \<Ztypecolon> \<nat>[b] \<rbrace>\<close>
+lemma op_const_word_\<phi>app:
+  \<open> \<^bold>p\<^bold>r\<^bold>o\<^bold>c op_const_int LENGTH('b) (unat n) \<lbrace> Void \<longmapsto> \<^bold>v\<^bold>a\<^bold>l n \<Ztypecolon> Word('b) \<rbrace> \<close>
   unfolding op_const_int_def Premise_def Synthesis_def
   by (rule, simp add: \<phi>expns)
+
+lemma
+  \<open> \<^bold>p\<^bold>r\<^bold>e\<^bold>m\<^bold>i\<^bold>s\<^bold>e n < 2 ^ LENGTH('b)
+\<Longrightarrow> \<^bold>p\<^bold>r\<^bold>o\<^bold>c op_const_int LENGTH('b::len) n \<lbrace> Void \<longmapsto> \<^bold>v\<^bold>a\<^bold>l n \<Ztypecolon> \<nat>('b) \<rbrace> \<close>
+  \<medium_left_bracket> have [simp]: \<open>unat (word_of_nat n :: 'b word) = n\<close> using \<phi> of_nat_inverse by blast 
+    ;; op_const_word[where 'b='b and n=\<open>of_nat n\<close>, simplified]
+  \<medium_right_bracket>. .
 
 lemma [\<phi>reason 1200
     for \<open>Synthesis_Parse (numeral ?n::nat) (?X :: ?'ret \<Rightarrow> assn)\<close>
@@ -312,6 +380,20 @@ lemma [\<phi>reason 1200
 subsubsection \<open>Integer Arithmetic\<close>
 
 paragraph \<open>Addition\<close>
+
+lemma op_add_word_\<phi>app:
+  \<open> \<^bold>p\<^bold>r\<^bold>o\<^bold>c op_add LENGTH('b) (\<phi>V_pair vy vx) \<lbrace> x \<Ztypecolon> \<^bold>v\<^bold>a\<^bold>l[vx] Word\<heavy_comma> y \<Ztypecolon> \<^bold>v\<^bold>a\<^bold>l[vy] Word \<longmapsto> \<^bold>v\<^bold>a\<^bold>l x + y \<Ztypecolon> Word \<rbrace>\<close>
+  for x :: \<open>'b::len word\<close>
+  unfolding op_add_def Premise_def
+  by (cases vx; cases vy; simp, rule, rule, simp add: \<phi>expns, rule,
+      simp add: \<phi>expns, rule, simp add: \<phi>expns unat_word_ariths)
+
+lemma
+  \<open> \<^bold>p\<^bold>r\<^bold>e\<^bold>m\<^bold>i\<^bold>s\<^bold>e x + y < 2 ^ LENGTH('b)
+\<Longrightarrow> \<^bold>p\<^bold>r\<^bold>o\<^bold>c op_add LENGTH('b::len) (\<phi>V_pair vy vx) \<lbrace> x \<Ztypecolon> \<^bold>v\<^bold>a\<^bold>l[vx] \<nat>('b)\<heavy_comma> y \<Ztypecolon> \<^bold>v\<^bold>a\<^bold>l[vy] \<nat>('b) \<longmapsto> \<^bold>v\<^bold>a\<^bold>l x + y \<Ztypecolon> \<nat>('b) \<rbrace> \<close>
+  \<medium_left_bracket> $vx $vy op_add_word[where 'b='b]
+  \<medium_right_bracket> using \<phi>
+    by (metis of_nat_add of_nat_inverse) .
 
 lemma op_add[\<phi>overload +]:
   \<open> \<^bold>p\<^bold>r\<^bold>e\<^bold>m\<^bold>i\<^bold>s\<^bold>e x + y < 2 ^ Big b
